{
 "cells": [
  {
   "cell_type": "markdown",
   "metadata": {},
   "source": [
    "# Some notable covariance matrix derivatives\n",
    "\n",
    "Reference: [Matrix Calculus Proofs](http://www.ee.ic.ac.uk/hp/staff/dmb/matrix/proof002.html)\n",
    "\n",
    "## Basic properties\n",
    "- Transpose: $dX^\\top = d(X^\\top) = (dX)^\\top$.\n",
    "- Inverse transpose: $X^{-\\top} = (X^{-1})^\\top = (X^\\top)^{-1}$.\n",
    "- Product rule: $d(XY) = (dX)Y + X(dY)$."
   ]
  },
  {
   "cell_type": "markdown",
   "metadata": {},
   "source": [
    "## Identities\n",
    "Let $\\mathbf{e_i}$ be the $i$-th column of the identity matrix and $L$ be the Cholesky decomposed matrix of a symmetric matrix $C$, _i.e._, $L$ is a lower triangular matrix and $C = LL^\\top$. The following holds.\n",
    "\n",
    "1. $\\frac{d}{dc_{ij}}C = \\mathbf{e_i}\\mathbf{e_j}^\\top$ where $\\mathbf{e_i}\\mathbf{e_j}^\\top$ is a matrix containing a 1 in position $i$, $j$ and zeros elsewhere.\n",
    "\n",
    "2. $dC^{-1} = -C^{-1}dC C^{-1}$.\n",
    "\n",
    "3. $\\frac{d}{dc_{ij}}C^{-1} = -C^{-1} \\mathbf{e_i} (C^{-\\top} \\mathbf{e_j}^\\top)^\\top$.\n",
    "\n",
    "4. $\\frac{d}{dC} \\mathbf{a}^\\top C^{-1} \\mathbf{b} = -C^{-1} \\mathbf{a} \\mathbf{b}^\\top C^{-1}$.\n",
    "\n",
    "5. $\\frac{d}{dL} \\mathbf{a}^\\top C^{-1} \\mathbf{b} = -L^{-\\top} L^{-1} (\\mathbf{b} \\mathbf{a}^\\top + \\mathbf{a} \\mathbf{b}^\\top) L^{-\\top}$."
   ]
  },
  {
   "cell_type": "markdown",
   "metadata": {},
   "source": [
    "## Proofs\n",
    "Let $I(x=X)$ be the indicator function\n",
    "\\begin{align*}\n",
    "    I(x = X) = \\begin{cases} 1 & x = X \\\\ 0 & \\text{otherwise} \\end{cases}\n",
    "\\end{align*}.\n",
    "\n",
    "1. $\\frac{d}{dc_{ij}}C = \\mathbf{e_i}\\mathbf{e_j}^\\top$.\n",
    "\n",
    "    \\begin{align*}\n",
    "        \\frac{d}{dc_{ij}}C &= \n",
    "        \\begin{bmatrix}\n",
    "            \\frac{d}{dc_{11}} c_{11} & \\ldots & \\frac{d}{dc_{1n}} c_{1n} \\\\\n",
    "            \\vdots & \\ddots & \\vdots \\\\\n",
    "            \\frac{d}{dc_{n1}} c_{n1} & \\ldots & \\frac{d}{dc_{nn}} c_{nn}\n",
    "        \\end{bmatrix} \\\\\n",
    "        &= \\begin{bmatrix}\n",
    "            I((i,j)=(1,1)) & \\ldots & I((i,j)=(1,n)) \\\\\n",
    "            \\vdots & \\ddots & \\vdots \\\\\n",
    "            I((i,j)=(n,1)) & \\ldots & I((i,j)=(n,n))\n",
    "        \\end{bmatrix} \\\\\n",
    "        &= \\begin{bmatrix}\n",
    "            I(i = 1) \\\\\n",
    "            \\vdots \\\\\n",
    "            I(i = n)\n",
    "        \\end{bmatrix}\n",
    "        \\begin{bmatrix}\n",
    "            I(j = 1) & \\ldots & I(j = n)\n",
    "        \\end{bmatrix} \\\\\n",
    "        &= \\mathbf{e_i} \\mathbf{e_j}^\\top.\n",
    "    \\end{align*}\n",
    "\n",
    "2. $dC^{-1} = -C^{-1}dC C^{-1}$.\n",
    "\n",
    "    \\begin{align*}\n",
    "        0 &= d(C C^{-1}) = (dC)C^{-1} + C(dC^{-1}) \\Rightarrow dC^{-1} = -C^{-1} dC C^{-1}.\n",
    "    \\end{align*}\n",
    "\n",
    "3. $\\frac{d}{dc_{ij}}C^{-1} = -C^{-1} \\mathbf{e_i} (C^{-\\top} \\mathbf{e_j}^\\top)^\\top$.\n",
    "\n",
    "    \\begin{align*}\n",
    "        \\frac{d}{dc_{ij}}C^{-1} &= -C^{-1} \\frac{d}{dc_{ij}}C C^{-1} = -C^{-1} \\mathbf{e_i} \\mathbf{e_j}^\\top C^{-1} = -C^{-1} \\mathbf{e_i} (C^{-\\top} \\mathbf{e_j}^\\top)^\\top.\n",
    "    \\end{align*}\n",
    "\n",
    "4. $\\frac{d}{dC} \\mathbf{a}^\\top C^{-1} \\mathbf{b} = -C^{-1} \\mathbf{a} \\mathbf{b}^\\top C^{-1}$.\n",
    "\n",
    "    \\begin{align*}\n",
    "        \\frac{d}{dc_{ij}} (\\mathbf{a}^\\top C^{-1} \\mathbf{b}) = \\mathbf{a}^\\top \\frac{d}{dc_{ij}}C^{-1} \\mathbf{b} &= \\underbrace{-\\mathbf{a}^\\top C^{-1} \\mathbf{e_i}}_{\\text{scalar}} \\underbrace{\\mathbf{e_j}^\\top C^{-1} \\mathbf{b}}_{\\text{scalar}} = \\mathbf{e_i}^\\top C^{-\\top} \\mathbf{a} \\mathbf{b}^\\top C^{-\\top} \\mathbf{e_j} = \\mathbf{e_i}^\\top C^{-1} \\mathbf{a} \\mathbf{b}^\\top C^{-1} \\mathbf{e_j}. \\\\\n",
    "        \\therefore \\frac{d}{dC} (\\mathbf{a}^\\top C^{-1} \\mathbf{b}) &= C^{-1} \\mathbf{a} \\mathbf{b}^\\top C^{-1}.\n",
    "    \\end{align*}\n",
    "\n",
    "5. $\\frac{d}{dL} \\mathbf{a}^\\top C^{-1} \\mathbf{b} = -L^{-\\top} L^{-1} (\\mathbf{b} \\mathbf{a}^\\top + \\mathbf{a} \\mathbf{b}^\\top) L^{-\\top}$.\n",
    "\n",
    "    \\begin{align*}\n",
    "        \\frac{d}{dl_{ij}} \\mathbf{a}^\\top C^{-1} \\mathbf{b} &= \\mathbf{a}^\\top \\frac{d}{dl_{ij}} (LL^\\top)^{-1} \\mathbf{b} = \\mathbf{a}^\\top \\frac{d}{dl_{ij}} (L^{-\\top} L^{-1}) \\mathbf{b} \\\\\n",
    "        &= \\mathbf{a}^\\top \\frac{d}{dl_{ij}} (L^{-\\top}) L^{-1} \\mathbf{b} + \\mathbf{a}^\\top L^{-\\top} \\frac{d}{dl_{ij}} (L^{-1}) \\mathbf{b} \\\\\n",
    "        &= \\mathbf{a}^\\top (\\frac{d}{dl_{ij}} L^{-1})^\\top L^{-1} \\mathbf{b} + \\mathbf{a}^\\top L^{-\\top} \\frac{d}{dl_{ij}} (L^{-1}) \\mathbf{b} \\\\\n",
    "        &= \\mathbf{a}^\\top (-L^{-1} \\mathbf{e_i} \\mathbf{e_j}^\\top L^{-1})^\\top L^{-1} \\mathbf{b} + \\mathbf{a}^\\top L^{-\\top} (-L^{-1} \\mathbf{e_i} \\mathbf{e_j}^\\top L^{-1}) \\mathbf{b} \\\\\n",
    "        &= -\\mathbf{a}^\\top (L^{-\\top} \\mathbf{e_j} \\mathbf{e_i}^\\top L^{-\\top}) L^{-1} \\mathbf{b} - \\mathbf{a}^\\top L^{-\\top} (L^{-1} \\mathbf{e_i} \\mathbf{e_j}^\\top L^{-1}) \\mathbf{b} \\\\\n",
    "        &= -\\underbrace{\\mathbf{a}^\\top L^{-\\top} \\mathbf{e_j}}_{\\text{scalar}} \\underbrace{\\mathbf{e_i}^\\top L^{-\\top} L^{-1} \\mathbf{b}}_{\\text{scalar}} - \\underbrace{\\mathbf{a}^\\top L^{-\\top} L^{-1} \\mathbf{e_i}}_{\\text{scalar}} \\underbrace{\\mathbf{e_j}^\\top L^{-1} \\mathbf{b}}_{\\text{scalar}} \\\\\n",
    "        &= -\\mathbf{e_i}^\\top L^{-\\top} L^{-1} \\mathbf{b} \\mathbf{a}^\\top L^{-\\top} \\mathbf{e_j} - \\mathbf{e_i}^\\top L^{-\\top} L^{-1} \\mathbf{a} \\mathbf{b}^\\top L^{-\\top} \\mathbf{e_j} \\\\\n",
    "        &= -\\mathbf{e_i}^\\top L^{-\\top} L^{-1} (\\mathbf{b} \\mathbf{a}^\\top + \\mathbf{a} \\mathbf{b}^\\top) L^{-\\top} \\mathbf{e_j}. \\\\\n",
    "        \\therefore \\frac{d}{dL} \\mathbf{a}^\\top C^{-1} \\mathbf{b} &= -L^{-\\top} L^{-1} (\\mathbf{b} \\mathbf{a}^\\top + \\mathbf{a} \\mathbf{b}^\\top) L^{-\\top}.\n",
    "    \\end{align*}"
   ]
  }
 ],
 "metadata": {
  "language_info": {
   "name": "python"
  }
 },
 "nbformat": 4,
 "nbformat_minor": 2
}
